adjustments, add more examples, rename file/theory

FOF_Examples.thy
@@ -1,17 +1,19 @@
 theory FOF_Examples
-  imports FOF_Base
+  imports FOF_Base FOF_Simplify FOF_Tseitin
 begin
+
+section \<open>eval_formula\<close>
 
 section \<open>tautology\<close>
 
 definition f1 :: "(string, string, string) formula" where
-"f1 = Or (Not (Pred ''A'' [Var ''x''])) (Pred ''A'' [Var ''x''])"
+"f1 = Or (Not (Pred ''a'' [Fun ''c'' []])) (Pred ''a'' [Fun ''c'' []])"
 
 definition f2 :: "(string, string, string) formula" where
 "f2 = Forall ''x'' (Equal (Fun ''f'' [Var ''x'']) (Fun  ''f'' [Var ''x'']))"
 
 definition f3 :: "(string, string, string) formula" where
-"f3 = And (Imp (Pred ''A'' []) (Pred ''A'' [])) (Imp (Pred ''B'' []) (Pred ''B'' []))"
+"f3 = Or (Imp (Pred ''a'' []) (Pred ''b'' [])) (Imp (Pred ''b'' []) (Pred ''a'' []))"
 
 definition f4 :: "(string, string, string) formula" where
 "f4 = Exists ''x'' (Exists ''y'' 
@@ -36,22 +38,22 @@ lemma f4_is_tautology:  "eval_formula f4 vI fI pI"
 section \<open>satisfiable\<close>
 
 definition f5 :: "(string, string, string) formula" where
-"f5 = Equiv (Pred ''A'' [Fun ''f'' [Var ''x'']]) (Pred ''B'' [Fun ''f'' [Var ''x'']])"
+"f5 = Equiv (Pred ''a'' []) (Equiv (Pred ''b'' []) (Pred ''c'' []))"
 
 definition f6 :: "(string, string, string) formula" where
-"f6 = Forall ''x'' (Pred ''A'' [Var ''x''])"
+"f6 = Forall ''x'' (Pred ''a'' [Var ''x''])"
 
 definition f7 :: "(string, string, string) formula" where
-"f7 = And (Forall ''x'' (Exists ''y'' (Equal (Var ''x'') (Var ''y'')))) (Pred ''A'' [Var ''z''])"
+"f7 = And (Forall ''x'' (Exists ''y'' (Equal (Var ''x'') (Var ''y'')))) (Pred ''a'' [])"
 
 definition f8 :: "(string, string, string) formula" where
-"f8 = Or (And (Pred ''A'' []) (Pred ''B'' [])) (And (Pred ''A'' []) (Not (Pred ''B'' [])))"
+"f8 = And (Pred ''a''  []) (Or (Pred ''b'' []) (Not (Pred ''c'' [])))"
 
 definition f9 :: "(string, string, string) formula" where
-"f9 = Imp (Pred ''B'' []) (Pred ''A'' [])"
+"f9 = Imp (Pred ''a'' []) (Pred ''b'' [])"
 
 definition f10 :: "(string, string, string) formula" where
-"f10 = Not (And (Pred ''A'' []) (Pred ''B'' []))"
+"f10 = Not (Pred ''a'' [Fun ''c'' []])"
 
 lemma f5_is_satisfiable: "\<exists>vI fI pI. eval_formula f5 vI fI pI" 
   unfolding f5_def Equiv_def Imp_def
@@ -59,25 +61,29 @@ lemma f5_is_satisfiable: "\<exists>vI fI pI. eval_formula f5 vI fI pI"
 
 lemma f5_is_not_tautology: "\<exists>pI vI fI. \<not> eval_formula f5 vI fI pI"
 proof (rule exI) 
-  let ?pI = "\<lambda> p args. (if p = ''A'' then True else False)"
+  let ?pI = "\<lambda> p args. (if p = ''b'' then False else True)"
   show "\<exists>vI fI. \<not> eval_formula f5 vI fI ?pI"
     unfolding f5_def Equiv_def Imp_def
     by simp
 qed
 
-lemma f6_is_satisfiable: "\<exists>vI pI. eval_formula f6 vI fI pI" 
+lemma "a \<longleftrightarrow> (b \<longleftrightarrow> c) = 
+  (\<not>a \<or> ((\<not>b \<or> c) \<and> (\<not>c \<or> b))) \<and> (\<not>((\<not>b \<or> c) \<and> (\<not>c \<or> b)) \<or> a)"
+  by satx
+
+lemma f6_is_satisfiable: "\<exists>pI. eval_formula f6 vI fI pI" 
   unfolding f6_def
   by auto
 
-lemma f6_is_not_tautology: "\<exists>vI pI. \<not> eval_formula f6 vI fI pI"
+lemma f6_is_not_tautology: "\<exists>pI. \<not> eval_formula f6 vI fI pI"
   unfolding f6_def
   by auto
 
-lemma f7_is_satisfiable: "\<exists>vI pI. eval_formula f7 vI fI pI" 
+lemma f7_is_satisfiable: "\<exists>pI. eval_formula f7 vI fI pI" 
   unfolding f7_def
   by auto
 
-lemma f7_is_not_tautology: "\<exists>vI pI. \<not> eval_formula f7 vI fI pI"
+lemma f7_is_not_tautology: "\<exists>pI. \<not> eval_formula f7 vI fI pI"
   unfolding f7_def
   by auto
 
@@ -95,7 +101,7 @@ lemma f9_is_satisfiable: "\<exists>pI. eval_formula f9 vI fI pI"
 
 lemma f9_is_not_tautology: "\<exists>pI. \<not> eval_formula f9 vI fI pI"
 proof (rule exI) 
-  let ?pI = "\<lambda> p args. (if p = ''B'' then True else False)"
+  let ?pI = "\<lambda> p args. (if p = ''a'' then True else False)"
   show "\<not> eval_formula f9 vI fI ?pI"
     unfolding f9_def Imp_def
     by simp
@@ -112,13 +118,13 @@ lemma f10_is_not_tautology: "\<exists>pI. \<not> eval_formula f10 vI fI pI"
 section \<open>unsatisfiable\<close>
 
 definition f11 :: "(string, string, string) formula" where
-"f11 = And (Not (Pred ''A'' [Var ''x''])) (Pred ''A'' [Var ''x''])"
+"f11 = And (Not (Pred ''a'' [])) (Pred ''a'' [])"
 
 definition f12 :: "(string, string, string) formula" where
-"f12 = Forall ''x'' (Not (Equal (Var ''x'') (Var ''x'')))"
+"f12 = Forall ''v'' (Not (Equal (Var ''v'') (Var ''v'')))"
 
 definition f13 :: "(string, string, string) formula" where
-"f13 = And (Pred ''A'' []) (And (Pred ''B'' []) (Not (Or (Pred ''A'' []) (Pred ''B'' []))))"
+"f13 = And (Pred ''a'' []) (And (Pred ''b'' []) (Not (Or (Pred ''a'' []) (Pred ''b'' []))))"
 
 definition f14 :: "(string, string, string) formula" where
 "f14 = Exists ''x'' (Exists ''y'' 
@@ -139,5 +145,74 @@ lemma unsatisfiable_f13: "\<not> eval_formula f13 vI fI pI"
 lemma unsatisfiable_f14: "\<not> eval_formula f14 vI fI pI"
   unfolding f14_def
   by simp
+
+
+section \<open>simp_formula\<close>
+
+definition f15 :: "(string, string, string) formula" where
+"f15 = Forall ''v'' (Or (And F (Pred ''a'' [])) (Not (Not (Pred ''b'' []))))"
+
+definition f16 :: "(string, string, string) formula" where
+"f16 = And (Pred ''a'' []) (Equal (Fun ''c1'' []) (Fun ''c2'' []))"
+
+lemma "eval_formula f15 vI fI pI = eval_formula (simp_formula f15) vI fI pI"
+  by (simp add: eval_formula_simp_formula_equiv_eval_formula)
+
+lemma "eval_formula f16 vI fI pI = eval_formula (simp_formula f16) vI fI pI"
+  by (simp add: eval_formula_simp_formula_equiv_eval_formula)
+
+lemma "simp_formula f16 = f16"
+  unfolding f16_def
+  by simp
+
+
+section \<open>tseitin_expansion\<close>
+
+definition fresh :: "nat set \<Rightarrow> nat" where
+  "fresh \<Sigma> = (if \<Sigma> = {} then 0 else Max \<Sigma> + 1)"
+
+definition f17 :: "(string, string, nat) formula" where
+"f17 = (Pred 0 [])"
+
+definition f18 :: "(string, string, nat) formula" where
+"f18 = (Not (Pred 0 []))"
+
+lemma "(\<exists>pI. eval_formula f17 vI fI pI) \<longleftrightarrow> 
+       (\<exists>pI. eval_formula (tseitin_expansion fresh f17) vI fI pI)"
+proof -
+  have fresh_spec: "\<And>\<V>. finite \<V> \<Longrightarrow> fresh \<V> \<notin> \<V>" 
+    unfolding fresh_def
+    by (metis Max.coboundedI add.commute
+        add_cancel_left_left all_not_in_conv le0
+        le_add_same_cancel1 order_antisym_conv
+        zero_neq_one)
+
+  have "is_nnf f17"
+    unfolding f17_def
+    by (simp add: PosPred)
+
+  show ?thesis
+    using tseitin_expansion_equisat[OF fresh_spec \<open>is_nnf f17\<close>]
+    by blast
+qed
+
+lemma "(\<exists>pI. eval_formula f18 vI fI pI) \<longleftrightarrow> 
+       (\<exists>pI. eval_formula (tseitin_expansion fresh f18) vI fI pI)"
+proof -
+  have fresh_spec: "\<And>\<V>. finite \<V> \<Longrightarrow> fresh \<V> \<notin> \<V>" 
+    unfolding fresh_def
+    by (metis Max.coboundedI add.commute
+        add_cancel_left_left all_not_in_conv le0
+        le_add_same_cancel1 order_antisym_conv
+        zero_neq_one)
+
+  have "is_nnf f18"
+    unfolding f18_def
+    by (simp add: NegPred)
+
+  show ?thesis
+    using tseitin_expansion_equisat[OF fresh_spec \<open>is_nnf f18\<close>]
+    by blast
+qed
 
 end
